Experiments/Test_Generator_Code_Export.thy
@@ -8,54 +8,30 @@ theory Test_Generator_Code_Export
 begin
 
 
-
-definition generate_test_suite_naive :: "(integer,integer,integer) fsm \<Rightarrow> integer \<Rightarrow> (integer\<times>integer) list set" where
-  "generate_test_suite_naive M m = calculate_test_suite_naive_as_io_sequences M (nat_of_integer m)"
-
-definition generate_test_suite_greedy :: "(integer,integer,integer) fsm \<Rightarrow> integer \<Rightarrow> (integer\<times>integer) list set" where
-  "generate_test_suite_greedy M m = calculate_test_suite_greedy_as_io_sequences M (nat_of_integer m)"
-
-
-subsection \<open>Counting Results\<close>
-
-definition count_maximal_repetition_sets_from_separators_naive :: "(integer,integer,integer) fsm \<Rightarrow> integer" where
-  "count_maximal_repetition_sets_from_separators_naive M = integer_of_nat (length (maximal_repetition_sets_from_separators_list_naive M))"
-
-definition count_maximal_repetition_sets_from_separators_greedy :: "(integer,integer,integer) fsm \<Rightarrow> integer" where
-  "count_maximal_repetition_sets_from_separators_greedy M = integer_of_nat (length (maximal_repetition_sets_from_separators_list_greedy M))"
-
-definition count_test_suite_naive :: "(integer,integer,integer) fsm \<Rightarrow> integer \<Rightarrow> integer" where
-  "count_test_suite_naive M m = integer_of_nat (card (generate_test_suite_naive M m))"
-
-definition count_test_suite_greedy :: "(integer,integer,integer) fsm \<Rightarrow> integer \<Rightarrow> integer" where
-  "count_test_suite_greedy M m = integer_of_nat (card (generate_test_suite_greedy M m))"
-
-
 subsection \<open>Generating the Test Suite as a List of Input-Output Sequences\<close>
 
 derive linorder list
 
 (* the call to sorted_list_of_set should not produce any significant overhead as the RBT-set is 
    already 'sorted' *)
-definition generate_test_suite_naive_list :: "(integer,integer,integer) fsm \<Rightarrow> integer \<Rightarrow> (integer\<times>integer) list list" where
-  "generate_test_suite_naive_list M m = sorted_list_of_set (calculate_test_suite_naive_as_io_sequences M (nat_of_integer m))"
+definition generate_test_suite_naive :: "(integer,integer,integer) fsm \<Rightarrow> integer \<Rightarrow> String.literal + (integer\<times>integer) list list" where
+  "generate_test_suite_naive M m = (case (calculate_test_suite_naive_as_io_sequences_with_assumption_check M (nat_of_integer m)) of
+    Inl err \<Rightarrow> Inl err |
+    Inr ts \<Rightarrow> Inr (sorted_list_of_set ts))"
 
-definition generate_test_suite_greedy_list :: "(integer,integer,integer) fsm \<Rightarrow> integer \<Rightarrow> (integer\<times>integer) list list" where
-  "generate_test_suite_greedy_list M m = sorted_list_of_set (calculate_test_suite_greedy_as_io_sequences M (nat_of_integer m))"
+definition generate_test_suite_greedy :: "(integer,integer,integer) fsm \<Rightarrow> integer \<Rightarrow> String.literal + (integer\<times>integer) list list" where
+  "generate_test_suite_greedy M m = (case (calculate_test_suite_greedy_as_io_sequences_with_assumption_check M (nat_of_integer m)) of
+    Inl err \<Rightarrow> Inl err |
+    Inr ts \<Rightarrow> Inr (sorted_list_of_set ts))"
 
 
 
-export_code generate_test_suite_naive 
-            generate_test_suite_greedy 
-            count_test_suite_naive 
-            count_maximal_repetition_sets_from_separators_naive 
-            count_test_suite_greedy 
-            count_maximal_repetition_sets_from_separators_greedy
+export_code Inl
             fsm_from_list 
             size 
             integer_of_nat 
-            generate_test_suite_naive_list
-            generate_test_suite_greedy_list
+            generate_test_suite_naive
+            generate_test_suite_greedy
 in Haskell module_name AdaptiveTestSuiteGenerator
 
 end
